theories/generic/utp_alphabet.thy
@@ -18,7 +18,7 @@ begin
 text {* Alphabets are encoded by finite sets of variables. *}
 
 definition WF_ALPHABET :: "'TYPE ALPHABET set" where
-"WF_ALPHABET = {a . finite a}"
+"WF_ALPHABET = {a . finite a (* \<and> (\<forall> x \<in> a. \<forall> y \<in> a. var_name x = var_name y \<longrightarrow> var_type x = var_type y) *)}"
 
 subsection {* Operators *}
 
@@ -32,6 +32,11 @@ definition out_alphabet ::
    'TYPE ALPHABET" ("out") where
 "out a = (a \<inter> DASHED)"
 
+definition homalph ::
+  "'TYPE ALPHABET \<Rightarrow>
+   'TYPE ALPHABET" where
+"homalph a = (in a \<union> undash ` out a) \<union> (out a \<union> dash ` in a)"
+
 subsection {* Restrictions *}
 
 definition COMPOSABLE ::
@@ -41,6 +46,9 @@ definition COMPOSABLE ::
  a2 \<in> WF_ALPHABET\<rbrakk> \<Longrightarrow>
  COMPOSABLE a1 a2 \<longleftrightarrow> (out a1) = dash ` (in a2)"
 
+definition HOMOGENEOUS :: "'TYPE ALPHABET \<Rightarrow> bool" where
+"HOMOGENEOUS a \<equiv> dash ` in a = out a"
+
 subsection {* Proof Support *}
 
 theorems utp_alphabet_simps =
@@ -48,6 +56,7 @@ theorems utp_alphabet_simps =
   DASHED_def
   DASHED_TWICE_def
   COMPOSABLE_def
+  HOMOGENEOUS_def
   in_alphabet_def
   out_alphabet_def
 
@@ -66,21 +75,21 @@ theorem WF_ALPHABET_insert [simp] :
 apply (simp add: WF_ALPHABET_def)
 done
 
-theorem WF_ALPHABET_union [simp] :
+theorem WF_ALPHABET_union [intro,simp] :
 "\<lbrakk>a1 \<in> WF_ALPHABET;
  a2 \<in> WF_ALPHABET\<rbrakk> \<Longrightarrow>
  a1 \<union> a2 \<in> WF_ALPHABET"
 apply (simp add: WF_ALPHABET_def)
 done
 
-theorem WF_ALPHABET_inter [simp] :
+theorem WF_ALPHABET_inter [intro,simp] :
 "\<lbrakk>a1 \<in> WF_ALPHABET;
  a2 \<in> WF_ALPHABET\<rbrakk> \<Longrightarrow>
  a1 \<inter> a2 \<in> WF_ALPHABET"
 apply (simp add: WF_ALPHABET_def)
 done
 
-theorem WF_ALPHABET_diff [simp] :
+theorem WF_ALPHABET_diff [intro,simp] :
 "\<lbrakk>a1 \<in> WF_ALPHABET;
  a2 \<in> WF_ALPHABET\<rbrakk> \<Longrightarrow>
  a1 - a2 \<in> WF_ALPHABET"
@@ -113,6 +122,11 @@ theorem WF_ALPHABET_out [simp, intro] :
 apply (simp add: out_alphabet_def)
 apply (simp add: WF_ALPHABET_def)
 done
+
+theorem WF_ALPHABET_homalph [simp, intro] :
+"a \<in> WF_ALPHABET \<Longrightarrow>
+ homalph a \<in> WF_ALPHABET"
+  by (simp add: homalph_def)
 
 subsection {* Simon's Theorems *}
 
@@ -167,7 +181,159 @@ done
 
 theorem out_alphabet_union [simp] :
 "out (a \<union> b) = out a \<union> out b"
-apply (auto simp: utp_alphabet_simps)
+by (auto simp: utp_alphabet_simps)
+
+theorem in_alphabet_ndash [simp] :
+"dash x \<notin> in a"
+by (simp add:utp_alphabet_simps dash_def)
+
+theorem out_alphabet_ndash [simp] : 
+"x \<in> out a \<Longrightarrow> dash x \<notin> out b"
+by (simp add:utp_alphabet_simps dash_def)
+
+theorem in_undashed [simp]:
+"in a \<subseteq> UNDASHED"
+  by (simp add: UNDASHED_def in_alphabet_def)
+
+theorem out_undashed [simp]:
+"out a \<subseteq> DASHED"
+  by (simp add: DASHED_def out_alphabet_def)
+
+theorem dash_undashed [simp]:
+"a \<subseteq> UNDASHED \<Longrightarrow> dash ` a \<subseteq> DASHED"
+  by (auto simp add: DASHED_def UNDASHED_def dash_def)
+
+theorem dash_dashed [simp]:
+"a \<subseteq> DASHED \<Longrightarrow> dash ` a \<subseteq> DASHED_TWICE"
+  by (auto simp add: DASHED_def DASHED_TWICE_def dash_def)
+
+theorem undash_dashed [simp]:
+"a \<subseteq> DASHED \<Longrightarrow> undash ` a \<subseteq> UNDASHED"
+  by (auto simp add: DASHED_def UNDASHED_def undash_def)
+
+theorem undash_dashed_twice [simp]:
+"a \<subseteq> DASHED_TWICE \<Longrightarrow> undash ` a \<subseteq> DASHED"
+  by (auto simp add: DASHED_def DASHED_TWICE_def undash_def)
+
+lemma out_undash: "a \<subseteq> UNDASHED \<union> DASHED \<Longrightarrow> out (undash ` a) = {}"
+  by (auto simp add:utp_alphabet_simps image_def undash_def)
+ 
+lemma in_undash:"a \<subseteq> UNDASHED \<union> DASHED \<Longrightarrow> in (undash ` a) = undash ` a"
+  by (auto simp add:utp_alphabet_simps undash_def image_def)
+
+lemma in_dash: "in (dash ` a) = {}"
+  by (auto simp add:utp_alphabet_simps dash_def image_def)
+
+lemma out_undash_out: "out (undash ` out a) = {}"
+  by (auto simp add:utp_alphabet_simps undash_def image_def)
+
+lemma out_dash_in: "out (dash ` in a) = dash ` in a"
+  by (auto simp add:utp_alphabet_simps dash_def image_def)
+
+theorem dash_undash[simp]: "dashes (name x) > 0 \<Longrightarrow> dash (undash x) = x"
+  apply(auto simp add:dash_def undash_def)
+  apply(smt NAME.surjective pair_collapse unit.exhaust)
 done
+
+theorem undash_dash[simp]: "undash (dash x) = x"
+  apply(auto simp add:dash_def undash_def)
+  apply(smt NAME.surjective pair_collapse unit.exhaust)
+done
+  
+lemma dash_undash_out: "dash ` undash ` out a = out a"
+  by (auto simp add:utp_alphabet_simps image_def)
+
+lemma undash_dash' : "undash ` dash ` a = a"
+  by (auto simp add:utp_alphabet_simps image_def)
+
+lemma in_out_disj[simp]: "in a \<inter> out b = {}"
+  by (auto simp add:in_alphabet_def out_alphabet_def DASHED_def UNDASHED_def)
+
+lemma in_out_complete: "a \<subseteq> UNDASHED \<union> DASHED \<Longrightarrow> in a \<union> out a = a"
+  by (auto simp add:utp_alphabet_simps)
+
+lemma override_out_in: "f \<oplus> (g \<oplus> h on (out a)) on (in b) = f \<oplus> g on (in b)"
+  by (metis Diff_triv in_out_disj override_on_cancel4)
+  
+lemma override_in_out: "f \<oplus> (g \<oplus> h on (in a)) on (out b) = f \<oplus> g on (out b)"
+  by (metis Diff_triv in_out_disj inf_commute override_on_cancel4)
+
+lemma homalph_in[simp]: "in (homalph a) = in a \<union> undash ` out a"
+  apply(simp add:homalph_def)
+  apply (smt Un_commute Un_empty_left in_alphabet_def in_dash inf_absorb2 inf_commute le_infI1 order_refl out_alphabet_def undash_dashed)
+done
+
+lemma homalph_out[simp]: "out (homalph a) = out a \<union> dash ` in a"
+  apply (simp add:homalph_def)
+  apply(metis out_dash_in out_undash_out sup_bot_left)
+done
+
+lemma dash_dist_inter: "dash ` (x \<inter> y) = dash ` x \<inter> dash ` y"
+  by (metis image_Int inj_dash)
+
+lemma dash_dist_union: "dash ` (x \<union> y) = dash ` x \<union> dash ` y"
+  by (metis image_Un)
+
+lemma homalph_homogeneous: "HOMOGENEOUS (homalph a)"
+  apply(simp add:HOMOGENEOUS_def)
+  apply (metis VAR.dash_undash_out image_Un sup_commute)
+done
+  
+lemma homogeneous_homalpha: "\<lbrakk> a \<subseteq> UNDASHED \<union> DASHED ; HOMOGENEOUS a \<rbrakk> \<Longrightarrow> homalph a = a"
+apply(simp add:HOMOGENEOUS_def homalph_def)
+  by (smt Int_Un_distrib Int_Un_distrib2 Un_absorb in_alphabet_def le_iff_inf out_alphabet_def undash_dash')
+
+lemma homalpha_dashes[simp]: "homalph a \<subseteq> UNDASHED \<union> DASHED"
+  by (metis Un_mono homalph_in homalph_out in_undashed out_undashed homalph_def)
+
+lemma homalpha_subset[simp]: "a \<subseteq> UNDASHED \<union> DASHED \<Longrightarrow> a \<subseteq> homalph a"
+proof (simp add:homalph_def)
+  assume "a \<subseteq> UNDASHED \<union> DASHED"
+  moreover hence "a = in a \<union> out a"
+    by (metis in_out_complete)
+  ultimately show "a \<subseteq> in a \<union> undash ` out a \<union> (out a \<union> dash ` in a)"
+    by auto
+qed
+
+
+lemma homalpha_mono[simp]: "a \<subseteq> b \<Longrightarrow> homalph a \<subseteq> homalph b"
+  by (auto simp add:homalph_def utp_alphabet_simps)
+
+(*
+lemma homalph_minus: "homalph (a - b) = homalph a - (b - homalph a)"
+proof
+  show "homalph (a - b) \<subseteq> homalph a - (b - homalph a)"
+    by (metis Diff_disjoint Diff_subset Diff_triv homalpha_mono)
+next
+  show "homalph a - (b - homalph a) \<subseteq> homalph (a - b)"
+    apply(auto)
+    apply(simp add:homalph_def)
+    apply(auto)
+    apply (metis DiffI Int_iff in_alphabet_def)
+    apply(simp add:image_def undash_def dash_def utp_alphabet_simps)
+    apply(auto)
+    apply(force)
+    
+  apply(clarify)
+  apply(fast)
+
+
+lemma homalpha_in_minus: "b \<subseteq> out a \<Longrightarrow> in (homalph (a - b)) = in (homalph a)"
+proof
+  assume assm:"b \<subseteq> out a"
+  thus "in (homalph (a - b)) \<subseteq> in (homalph a)"
+    by (metis Diff_subset VAR.homalpha_mono in_alphabet_def inf_mono set_eq_subset)
+
+next
+  assume assm:"b \<subseteq> out a"
+  thus "in (homalph a) \<subseteq> in (homalph (a - b))"
+    
+  
+ apply(simp add:homalph_def)
+ apply(safe)
+*)
+
 end
 end
+
+
