theories/generic/utp_gen_laws.thy
@@ -10,12 +10,13 @@ theory utp_gen_laws
 imports utp_eval_tactic (* "../algebra/alpha_boolean_algebra2" *)
 begin
 
+
 context GEN_PRED
 begin
 theorem AndP_intro :
 "\<lbrakk>p1 \<in> WF_ALPHA_PREDICATE;
  p2 \<in> WF_ALPHA_PREDICATE;
- (\<alpha> p1) = (\<alpha> p2);
+ \<alpha> p2 \<subseteq> \<alpha> p1;
  taut (p1 \<Rightarrow>p p2)\<rbrakk> \<Longrightarrow> p1 = (p1 \<and>p p2)"
 apply (utp_pred_taut_tac)
 apply (auto)
@@ -68,6 +69,33 @@ apply (utp_pred_eq_tac)
 apply (auto)
 done
 
+
+theorem OrP_RefP1:
+"\<lbrakk>p \<in> WF_ALPHA_PREDICATE;
+ q \<in> WF_ALPHA_PREDICATE;
+ \<alpha> p = \<alpha> q; p \<or>p q = q \<rbrakk> \<Longrightarrow>
+ q \<sqsubseteq> p"
+apply (utp_pred_taut_tac)
+apply(auto)
+done
+
+theorem OrP_RefP2:
+"\<lbrakk>p \<in> WF_ALPHA_PREDICATE;
+ q \<in> WF_ALPHA_PREDICATE;
+ \<alpha> p = \<alpha> q; q \<sqsubseteq> p \<rbrakk> \<Longrightarrow>
+ p \<or>p q = q"
+apply (utp_pred_taut_tac)
+apply(rule ballI)
+apply(erule ballE)
+apply(auto)
+done
+
+theorem OrP_RefP:
+"\<lbrakk>p \<in> WF_ALPHA_PREDICATE;
+ q \<in> WF_ALPHA_PREDICATE \<rbrakk> \<Longrightarrow>
+(\<alpha> p = \<alpha> q \<and> p \<or>p q = p) = (\<alpha> p = \<alpha> q \<and> p \<sqsubseteq> q)"
+  by (metis OrP_RefP1 OrP_RefP2 OrP_comm)
+
 (*
 abbreviation "GEN_PRED_algebra \<equiv>
  \<lparr> alpha_boolean_algebra.carrier = WF_ALPHA_PREDICATE,
@@ -78,7 +106,7 @@ abbreviation "GEN_PRED_algebra \<equiv>
    compl = NotP,
    top = TrueP,
    bot = FalseP,
-   ble = (\<lambda> x y. Refinement y x) \<rparr>"
+   ble = (\<lambda> x y. (\<alpha> x = \<alpha> y \<and> y \<sqsubseteq> x)) \<rparr>"
 end
 
 subsection {* Sublocale @{term alpha_boolean_algebra} *}
@@ -92,19 +120,28 @@ sublocale GEN_PRED \<subseteq> alpha_boolean_algebra "GEN_PRED_algebra" where
 "compl GEN_PRED_algebra = NotP"  and
 "top GEN_PRED_algebra = TrueP" and
 "bot GEN_PRED_algebra = FalseP" and
-"ble GEN_PRED_algebra = (\<lambda> x y. Refinement y x)"d
+"ble GEN_PRED_algebra = (\<lambda> x y. (\<alpha> x = \<alpha> y \<and> y \<sqsubseteq> x))"
 apply(unfold_locales)
 apply(simp_all)
-apply(utp_pred_eq_tac)+
-apply(utp_pred_taut_tac)
-apply(auto)
-apply(erule_tac ballE)+
-apply(auto)
+apply(utp_pred_eq_tac)
+apply(utp_pred_eq_tac)
+apply(utp_pred_eq_tac)
+apply(utp_pred_eq_tac)
+apply (metis OrP_RefP OrP_comm)
 apply(smt OrP_assoc)
 apply(smt OrP_comm)
 apply(metis OrP_identity set_eq_subset)
 apply(smt OrP_AndP_dist)
 done
+
+context GEN_PRED
+begin
+
+thm Upper_mem_cong
+
+
+end
 *)
+
 end
 end
