theories/theories/utp_rel.thy
@@ -7,8 +7,18 @@
 header {* Relational Predicates *}
 
 theory utp_rel
-imports "../generic/utp_generic"
+imports "../generic/utp_generic" "../generic/utp_expression"
 begin
+
+type_synonym ('VALUE, 'TYPE) ASSIGN = "('TYPE VAR * ('VALUE, 'TYPE) ALPHA_EXPRESSION)"
+type_synonym ('VALUE, 'TYPE) ASSIGNMENT = "('VALUE,'TYPE) ASSIGN list"
+
+definition assign_var :: "('VALUE, 'TYPE) ASSIGN \<Rightarrow> 'TYPE VAR" where
+"assign_var \<equiv> fst"
+
+definition assign_value :: "('VALUE, 'TYPE) ASSIGN \<Rightarrow> ('VALUE, 'TYPE) ALPHA_EXPRESSION" where
+"assign_value \<equiv> snd"
+
 
 context GEN_PRED
 begin
@@ -36,12 +46,11 @@ definition SS2 :: "'TYPE VAR \<Rightarrow> 'TYPE VAR" where
  if dashes (name v) = 2 then undash (undash v) else v)"
 
 subsection {* Relational Operators *}
-
+      
 definition SkipR ::
   "'TYPE ALPHABET \<Rightarrow> ('VALUE, 'TYPE) ALPHA_PREDICATE" ("\<Pi>_") where
-"a \<in> WF_ALPHABET \<and>
- a \<subseteq> UNDASHED \<longrightarrow>
- \<Pi> a = LiftP (a \<union> dash ` a) (\<lambda> b . \<forall> x \<in> a . b x = b (dash x))"
+"a \<in> WF_ALPHABET \<longrightarrow>
+ \<Pi> a = LiftP (homalph a) (\<lambda> b . \<forall> x \<in> in (homalph a) . b x = b (dash x))"
 
 definition CondR ::
   "('VALUE, 'TYPE) ALPHA_PREDICATE \<Rightarrow>
@@ -64,11 +73,65 @@ definition SemiR ::
  COMPOSABLE (\<alpha> r1) (\<alpha> r2) \<longrightarrow>
  r1 ; r2 = (\<exists>-p dash ` (out (\<alpha> r1)) . r1[SS1] \<and>p r2[SS2])"
 
+definition SemiB :: "('VALUE, 'TYPE) ALPHA_PREDICATE
+                    \<Rightarrow> ('VALUE, 'TYPE) ALPHA_PREDICATE
+                    \<Rightarrow> ('VALUE, 'TYPE) ALPHA_PREDICATE" (infixr ";\<^sub>B" 140) where
+"p \<in> WF_RELATION \<and> q \<in> WF_RELATION \<and>
+ COMPOSABLE (\<alpha> p) (\<alpha> q) \<longrightarrow>
+  SemiB p q = ((in (\<alpha> p)) \<union> (out (\<alpha> q))
+             ,{(b \<oplus> b1 on in (\<alpha> p)) \<oplus> b2 on out (\<alpha> q) 
+              | b1 b2 b. b1 \<in> \<beta> p \<and> b2 \<in> \<beta> q \<and> b \<in> WF_BINDING
+                     \<and> (\<forall>x \<in> in(\<alpha> q). b1 (dash x) = b2 x) })"
+
+inductive WF_ASSIGNMENT :: "'TYPE ALPHABET \<Rightarrow> (('VALUE, 'TYPE) ASSIGNMENT) \<Rightarrow> bool" 
+where
+"WF_ASSIGNMENT a []" | 
+"\<lbrakk> dash (assign_var v) \<in> a
+ ; expr_type (assign_value v) = var_type (assign_var v)
+ ; assign_var v \<in> UNDASHED
+ ; assign_value v \<in> WF_ALPHA_EXPR
+ ; \<alpha>e (assign_value v) \<subseteq> a
+ ; \<alpha>e (assign_value v) \<subseteq> UNDASHED
+ ; WF_ASSIGNMENT (a - {dash (assign_var v)}) vs \<rbrakk> 
+ \<Longrightarrow> WF_ASSIGNMENT a (v # vs)"
+
+inductive_cases WF_ASSIGNMENT_cons' [elim!]: "WF_ASSIGNMENT a (v # vs)"
+
+thm WF_ASSIGNMENT_cons'
+
+lemma WF_ASSIGNMENT_cons[elim!]:
+"\<lbrakk>(v # vs) \<in> WF_ASSIGNMENT a;
+ \<lbrakk>dash (assign_var v) \<in> a; expr_type (assign_value v) = type (assign_var v); assign_var v \<in> UNDASHED;
+  assign_value v \<in> WF_ALPHA_EXPR; \<alpha>e (assign_value v) \<subseteq> a; \<alpha>e (assign_value v) \<subseteq> UNDASHED; vs \<in> WF_ASSIGNMENT (a - {dash (assign_var v)})\<rbrakk>
+ \<Longrightarrow> P\<rbrakk>
+\<Longrightarrow> P"
+  by (auto simp add:mem_def)
+
+primrec mkAssign :: "('VALUE, 'TYPE) ASSIGNMENT \<Rightarrow> 'TYPE ALPHABET \<Rightarrow> ('VALUE, 'TYPE) ALPHA_PREDICATE" where
+"mkAssign [] a = \<Pi> a" |
+"mkAssign (v # vs) a = ((VarE (dash (assign_var v)) =p assign_value v) \<and>p mkAssign vs (a - {dash (assign_var v)}))"
+
+definition AssignR :: "('VALUE, 'TYPE) ASSIGNMENT \<Rightarrow> 'TYPE ALPHABET \<Rightarrow> ('VALUE, 'TYPE) ALPHA_PREDICATE" where
+"xs \<in> WF_ASSIGNMENT a \<and> a \<in> WF_ALPHABET 
+ \<and> a \<subseteq> UNDASHED \<union> DASHED \<and> HOMOGENEOUS a \<longrightarrow> 
+ AssignR xs a = mkAssign xs a"
+
+abbreviation AssignR_1 :: "'TYPE VAR \<Rightarrow> 'TYPE ALPHABET \<Rightarrow> ('VALUE, 'TYPE) ALPHA_EXPRESSION \<Rightarrow> ('VALUE, 'TYPE) ALPHA_PREDICATE" ("_ :=\<^bsub>_ \<^esub>_") where
+"AssignR_1 x a e \<equiv> AssignR [(x,e)] a"
+
+(* ("_ :=\<^bsub>_ \<^esub>_") *)
+
 text {* Configure theorems for the automatic proof tactic. *}
 
 declare SkipR_def [eval]
 declare CondR_def [eval]
 declare SemiR_def [eval]
+declare AssignR_def [eval]
+
+lemma SemiR_eval[eval]: 
+"\<lbrakk> p \<in> WF_RELATION; q \<in> WF_RELATION; COMPOSABLE (\<alpha> p) (\<alpha> q) \<rbrakk>
+ \<Longrightarrow> EvalP (p ; q) b = (EvalP (\<exists>-p dash ` (out (\<alpha> p)) . (p[SS1] \<and>p q[SS2])) b)"
+  by (simp add:SemiR_def)
 
 subsection {* Theorems *}
 
@@ -88,25 +151,12 @@ done
 
 declare WF_RELATION_alphabet [eval]
 
+theorem WF_RELATION_UNDASHED_DASHED :
+"p \<in> WF_RELATION \<Longrightarrow> \<alpha> p \<subseteq> UNDASHED \<union> DASHED"
+  by (simp add: WF_RELATION_def)
+
 subsubsection {* Substitutions *}
 
-theorem SS1_VAR_SUBST [simp] :
-"SS1 \<in> VAR_SUBST"
-apply (simp add: SS1_def_raw)
-apply (simp add: VAR_SUBST_def)
-apply (simp_all add: dash_def undash_def)
-apply (rule bijI)
-apply (rule injI)
-oops
-
-theorem SS2_VAR_SUBST [simp] :
-"SS2 \<in> VAR_SUBST"
-apply (simp add: SS2_def_raw)
-apply (simp add: VAR_SUBST_def)
-apply (simp_all add: dash_def undash_def)
-apply (rule bijI)
-apply (rule injI)
-oops
 
 text {* Simon's Theorems *}
 
@@ -144,6 +194,15 @@ apply (force simp add: SS1_def DASHED_def UNDASHED_def
   Un_def in_alphabet_def out_alphabet_def image_def SS1_def)
 done
 
+theorem SS1_invol:
+"SS1 \<circ> SS1 = id"
+apply(auto simp add: comp_def SS1_def id_def)
+apply(rule ext)
+apply(case_tac "dashes(name x) = 0")
+apply(auto)
+apply(auto simp add:undash_def dash_def intro:NAME.equality NAME.surjective unit.exhaust pairI)
+done
+
 theorem SS2_dashes[simp, intro, eval] :
 "a \<subseteq> UNDASHED \<union> DASHED \<Longrightarrow> SS2 ` a = (dash ` dash ` in a) \<union> (out a)"
 apply (auto simp add: SS2_def DASHED_def UNDASHED_def
@@ -152,19 +211,189 @@ apply (simp_all add:image_def SS2_def)
 apply (rule bexI, auto)+
 done
 
+theorem SS2_invol:
+"SS2 \<circ> SS2 = id"
+apply(auto simp add: SS2_def id_def comp_def)
+apply(rule ext)
+apply(case_tac "dashes(name x) = 0")
+apply(auto)
+apply(auto simp add:undash_def dash_def intro:NAME.equality NAME.surjective unit.exhaust pairI)
+apply(case_tac x)
+apply(case_tac a)
+apply(auto)
+done
+
+theorem SubstB_SS1_beta_equiv[simp]:
+"\<lbrakk> b1 \<in> WF_BINDING; b2 \<in> WF_BINDING; a \<subseteq> UNDASHED \<rbrakk> \<Longrightarrow> 
+  (SubstB SS1 b1 \<cong> b2 on a) = (b1 \<cong> b2 on a)" 
+  apply(auto simp add: SubstB_def UNDASHED_def beta_equiv_def)
+  apply(erule_tac x="x" in ballE)
+  apply(subgoal_tac "dashes (name x) = 0")
+  apply(auto)
+  apply (smt SS1_VAR_SUBST SS1_def VAR_SUBST_inv_ss)
+  apply(erule_tac x="x" in ballE)
+  apply(subgoal_tac "dashes (name x) = 0")
+  apply(auto)
+  apply(smt SS1_VAR_SUBST SS1_def VAR_SUBST_inv_ss)
+done  
+
+theorem SubstB_SS2_beta_equiv[simp]:
+"\<lbrakk> b1 \<in> WF_BINDING; b2 \<in> WF_BINDING; a \<subseteq> DASHED \<rbrakk> \<Longrightarrow> 
+  (SubstB SS2 b1 \<cong> b2 on a) = (b1 \<cong> b2 on a)" 
+  apply(auto simp add: SubstB_def DASHED_def beta_equiv_def)
+  apply(erule_tac x="x" in ballE)
+  apply(subgoal_tac "dashes (name x) = 1")
+  apply(auto)
+  apply (smt SS2_VAR_SUBST SS2_def VAR_SUBST_inv_ss)
+  apply(erule_tac x="x" in ballE)
+  apply(subgoal_tac "dashes (name x) = 1")
+  apply(auto)
+  apply(smt SS2_VAR_SUBST SS2_def VAR_SUBST_inv_ss)
+done  
+
+theorem SS1_d0: "x \<in> UNDASHED \<Longrightarrow> SS1 x = x"
+  by (simp add:SS1_def UNDASHED_def)
+
+theorem SS1_d1: "x \<in> DASHED \<Longrightarrow> SS1 x = dash x"
+  by (simp add:SS1_def DASHED_def)
+
+theorem SS1_d2: "x \<in> DASHED_TWICE \<Longrightarrow> SS1 x = undash x"
+  by (simp add:SS1_def DASHED_TWICE_def)
+
+theorem SS2_d0: "x \<in> UNDASHED \<Longrightarrow> SS2 x = dash (dash x)"
+  by (simp add:SS2_def UNDASHED_def)
+
+theorem SS2_d1: "x \<in> DASHED \<Longrightarrow> SS2 x = x"
+  by (simp add:SS2_def DASHED_def)
+
+theorem SS2_d2: "x \<in> DASHED_TWICE \<Longrightarrow> SS2 x = undash (undash x)"
+  by (simp add:SS2_def DASHED_TWICE_def)
+
+theorem SS1_undashed: "a \<subseteq> UNDASHED \<Longrightarrow> SS1 ` a \<subseteq> UNDASHED"
+  by (smt SS1_d0 image_subsetI subsetD)
+
+theorem SS1_dashed: "a \<subseteq> DASHED \<Longrightarrow> SS1 ` a \<subseteq> DASHED_TWICE"
+  apply(rule_tac image_subsetI)
+  apply(drule subsetD)
+  apply(auto simp add:SS1_d1 DASHED_TWICE_def DASHED_def dash_def)
+done
+
+theorem SS1_inv_d2[simp]:
+"x \<in> DASHED_TWICE \<Longrightarrow> inv SS1 x = undash x"
+apply(simp add:inv_def)
+apply(rule some_equality)
+apply(subgoal_tac "dashes (name (undash x)) = 1")
+apply(simp add:SS1_def DASHED_TWICE_def)
+apply(simp add:undash_def DASHED_TWICE_def)
+apply(auto simp add:SS1_def DASHED_TWICE_def)
+apply(simp add:undash_def)
+done
+
+theorem SS2_inv_d2[simp]:
+"x \<in> DASHED_TWICE \<Longrightarrow> inv SS2 x = undash (undash x)"
+apply(simp add:inv_def)
+apply(rule some_equality)
+apply(subgoal_tac "dashes (name (undash (undash x))) = 0")
+apply(simp add:SS2_def)
+apply(subgoal_tac "dashes (name (undash x)) = 1")
+apply(simp add:DASHED_TWICE_def)
+apply(simp add:undash_def DASHED_TWICE_def)
+apply(auto simp add:SS2_def DASHED_TWICE_def)
+apply(simp add:undash_def DASHED_TWICE_def)
+apply(simp add:undash_def DASHED_TWICE_def)
+done
+
+lemma SS1_beta_equiv_in:
+assumes "p \<in> WF_ALPHA_PREDICATE" "bp \<in> \<beta> p" "a \<subseteq> in (\<alpha> p)"
+shows "SubstB SS1 bp \<cong> bp on a"
+  by (smt SubstB_SS1_beta_equiv in_undashed WF_BINDING_predicate assms beta_equiv_def beta_equiv_subset)
+
+lemma SS1_override_in:
+assumes "p \<in> WF_ALPHA_PREDICATE" "bp \<in> \<beta> p" "a \<subseteq> in (\<alpha> p)"
+shows "SubstB SS1 bp \<oplus> bp on a = SubstB SS1 bp"
+  by (metis SS1_beta_equiv_in assms beta_equiv_override)
+
+(* Unfortunately I have to specialise this, as the First Order ATPs don't seem
+   to cope with subset proofs very well (even trivial ones) *)
+lemma SS1_override_in':
+"\<lbrakk> p \<in> WF_ALPHA_PREDICATE; bp \<in> \<beta> p \<rbrakk> \<Longrightarrow>
+   SubstB SS1 bp \<oplus> bp on in (\<alpha> p) = SubstB SS1 bp"
+  by (auto intro: SS1_override_in)
+
+lemma SS2_beta_equiv_out:
+assumes "p \<in> WF_ALPHA_PREDICATE" "bp \<in> \<beta> p" "a \<subseteq> out (\<alpha> p)"
+shows "SubstB SS2 bp \<cong> bp on a"
+  by (smt SubstB_SS2_beta_equiv out_undashed WF_BINDING_predicate assms beta_equiv_def beta_equiv_subset)
+
+lemma SS2_override_out:
+assumes "p \<in> WF_ALPHA_PREDICATE" "bp \<in> \<beta> p" "a \<subseteq> out (\<alpha> p)"
+shows "SubstB SS2 bp \<oplus> bp on a = SubstB SS2 bp"
+  by (metis SS2_beta_equiv_out assms beta_equiv_override)
+
+lemma SS2_override_out':
+"\<lbrakk> p \<in> WF_ALPHA_PREDICATE; bp \<in> \<beta> p  \<rbrakk> \<Longrightarrow>
+   SubstB SS2 bp \<oplus> bp on out (\<alpha> p) = SubstB SS2 bp"
+  by (auto intro: SS2_override_out)
+
+lemma SS1_SS2_overlap:
+assumes "p \<in> WF_ALPHA_PREDICATE" "q \<in> WF_ALPHA_PREDICATE" "bp \<in> \<beta> p" "bq \<in> \<beta> q"
+        "\<forall>x\<in>in (\<alpha> q). bp (dash x) = bq x" 
+shows "SubstB SS1 bp \<cong> SubstB SS2 bq on (dash ` dash ` in (\<alpha> q))"
+proof -
+  from assms have "bp \<in> WF_BINDING" "bq \<in> WF_BINDING"
+    by (auto simp add:WF_ALPHA_PREDICATE_def WF_BINDING_SET_def)    
+
+  with assms show ?thesis
+    by (simp add:beta_equiv_def SubstB_def) 
+       (metis SS1_inv_d2 SS2_inv_d2 VAR.in_undashed dash_dashed dash_undashed imageI subsetD undash_dash)
+qed
+
+lemma SS1_SS2_alpha_union1:
+"\<lbrakk> a \<in> WF_ALPHABET; b \<in> WF_ALPHABET ; COMPOSABLE a b
+ ; a \<subseteq> UNDASHED \<union> DASHED; b \<subseteq> UNDASHED \<union> DASHED \<rbrakk> \<Longrightarrow> 
+  SS1 ` a \<union> SS2 ` b = SS1 ` a \<union> out b"
+  by auto
+
+lemma SS1_SS2_alpha_union2:
+"\<lbrakk> a \<in> WF_ALPHABET; b \<in> WF_ALPHABET ; COMPOSABLE a b
+ ; a \<subseteq> UNDASHED \<union> DASHED; b \<subseteq> UNDASHED \<union> DASHED \<rbrakk> \<Longrightarrow> 
+  SS1 ` a \<union> SS2 ` b = in a \<union> SS2 ` b"
+  by auto
+
+lemma SS1_SubstB:
+  "b \<in> WF_BINDING \<Longrightarrow> SubstB SS1 (SubstB SS1 b) = b"
+  by (metis SS1_VAR_SUBST SS1_invol SubstB_invol)
+
+lemma SS2_SubstB:
+  "b \<in> WF_BINDING \<Longrightarrow> SubstB SS2 (SubstB SS2 b) = b"
+  by (metis SS2_VAR_SUBST SS2_invol SubstB_invol)
+
+lemma SS1_image_invol:
+  "SS1 ` SS1 ` a = a"
+  by (metis image_compose SS1_invol image_id)
+
+lemma SS2_image_invol:
+  "SS2 ` SS2 ` a = a"
+  by (metis image_compose SS2_invol image_id)
+
 subsubsection {* Alphabet Theorems *}
 
-theorem WF_BINDING_FUN_SkipR [simp] :
-"(\<lambda> b . \<forall> x \<in> a . f (b x) (b (dash x))) \<in> WF_BINDING_FUN (a \<union> dash ` a)"
+theorem WF_BINDING_FUN_SkipR [simplified,simp] :
+"(\<lambda> b . \<forall> x \<in> in (homalph a) . f (b x) (b (dash x))) \<in> WF_BINDING_FUN (homalph a)"
 apply (simp add: WF_BINDING_FUN_def)
 apply (simp add: beta_equiv_def)
+apply(subgoal_tac "\<forall>x\<in>in (homalph a).x \<in> homalph a")
+apply(subgoal_tac "\<forall>x\<in>in (homalph a).dash x \<in> homalph a")
+apply(auto)
+apply(auto simp add:homalph_def)
+apply(metis VAR.dash_undash_out image_iff)
 done
 
 theorem SkipR_alphabet [simp] :
-"\<lbrakk>a \<in> WF_ALPHABET;
- a \<subseteq> UNDASHED\<rbrakk> \<Longrightarrow>
- \<alpha> (\<Pi> a) = a \<union> dash ` a"
+"\<lbrakk>a \<in> WF_ALPHABET; a \<subseteq> UNDASHED \<union> DASHED; HOMOGENEOUS a \<rbrakk> \<Longrightarrow>
+ \<alpha> (\<Pi> a) = a"
 apply (simp add: SkipR_def)
+apply(simp add:homogeneous_homalpha)
 done
 
 theorem CondR_alphabet [simp]:
@@ -185,6 +414,8 @@ assumes assm:
   "r2 \<in> WF_RELATION"
   "COMPOSABLE (\<alpha> r1) (\<alpha> r2)"
 shows "\<alpha> (r1 ; r2) = in (\<alpha> r1) \<union> out (\<alpha> r2)"
+apply(insert assm)
+apply(utp_pred_eq_tac)
 proof (insert assm, utp_pred_eq_tac)
   from assm have
     "\<alpha> r1 \<in> WF_ALPHABET"
@@ -201,16 +432,30 @@ proof (insert assm, utp_pred_eq_tac)
   done
 qed
 
+lemma SemiR_in_alpha: "\<lbrakk> p \<in> WF_RELATION; q \<in> WF_RELATION; COMPOSABLE (\<alpha> p) (\<alpha> q) \<rbrakk> \<Longrightarrow> in (\<alpha> (p ; q)) = in (\<alpha> p)"
+  by simp
+
+lemma SemiR_out_alpha: "\<lbrakk> p \<in> WF_RELATION; q \<in> WF_RELATION; COMPOSABLE (\<alpha> p) (\<alpha> q) \<rbrakk> \<Longrightarrow> out (\<alpha> (p ; q)) = out (\<alpha> q)"
+  by simp
+
+theorem SemiB_alphabet [simp] :
+assumes assm:
+  "r1 \<in> WF_RELATION"
+  "r2 \<in> WF_RELATION"
+  "COMPOSABLE (\<alpha> r1) (\<alpha> r2)"
+shows "\<alpha> (r1 ;\<^sub>B r2) = in (\<alpha> r1) \<union> out (\<alpha> r2)"
+  apply(insert assms)
+  apply(simp add:SemiB_def)
+done
+
 subsubsection {* Closure Theorems *}
 
 theorem SkipR_closure [simp] :
 "\<lbrakk>a \<in> WF_ALPHABET;
- a \<subseteq> UNDASHED\<rbrakk> \<Longrightarrow>
+  a \<subseteq> UNDASHED \<union> DASHED\<rbrakk> \<Longrightarrow>
  (\<Pi> a) \<in> WF_RELATION"
 apply (simp add: SkipR_def)
 apply (simp add: WF_RELATION_def)
-apply (simp add: UNDASHED_def DASHED_def)
-apply (auto simp add: dash_def)
 done
 
 theorem CondR_closure [simp] :
@@ -238,6 +483,194 @@ proof -
     by (auto simp add: WF_RELATION_def in_alphabet_def out_alphabet_def)
 qed
 
+lemma SemiB_wfalpha[intro]: "\<lbrakk> p \<in> WF_RELATION; q \<in> WF_RELATION; COMPOSABLE (\<alpha> p) (\<alpha> q) \<rbrakk> \<Longrightarrow>
+                      \<alpha> (SemiB p q) \<in> WF_ALPHABET"
+  by (simp add:SemiB_def)
+
+lemma SemiB_closure: 
+assumes "p \<in> WF_RELATION" "q \<in> WF_RELATION" "COMPOSABLE (\<alpha> p) (\<alpha> q)"
+shows "SemiB p q \<in> WF_RELATION"
+proof -
+  from assms have "\<alpha> (p ;\<^sub>B q) \<in> WF_ALPHABET"
+    by auto
+
+  also from assms have "\<beta> (p ;\<^sub>B q) \<in> WF_BINDING_SET (\<alpha> (p ;\<^sub>B q))"
+    apply(simp add:WF_BINDING_SET_def SemiB_def)
+    apply(auto)
+    apply(metis WF_BINDING_override WF_BINDING_predicate WF_RELATION_WF_ALPHA_PREDICATE)
+    apply(smt VAR.override_out_in beta_equiv_comm beta_equiv_override beta_equiv_override_3 beta_equiv_trans beta_equiv_union)
+  done
+
+  moreover from assms have "\<alpha> (p ;\<^sub>B q) \<subseteq> UNDASHED \<union> DASHED"
+    by (auto simp add:SemiB_def in_alphabet_def out_alphabet_def)
+   
+  ultimately show ?thesis
+    by (auto simp only:WF_RELATION_def WF_ALPHA_PREDICATE_def)
+
+qed
+
+lemma mkAssign_closure[simp]:
+"\<lbrakk> vs \<in> WF_ASSIGNMENT a; a \<in> WF_ALPHABET; a \<subseteq> UNDASHED \<union> DASHED \<rbrakk>
+   \<Longrightarrow> mkAssign vs a \<in> WF_RELATION"
+proof (induct vs arbitrary: a)
+  case Nil
+  thus ?case 
+    by simp
+
+next
+  case (Cons v vs)
+
+  moreover from `v # vs \<in> WF_ASSIGNMENT a` have "vs \<in> WF_ASSIGNMENT (a - {dash (assign_var v)})"
+    by auto
+
+  moreover from `a \<in> WF_ALPHABET` have alp:"a - {dash (assign_var v)} \<in> WF_ALPHABET"
+    by (simp add:WF_ALPHABET_def)
+
+  moreover from `a \<subseteq> UNDASHED \<union> DASHED` have ud:"a - {dash (assign_var v)} \<subseteq> UNDASHED \<union> DASHED"
+    by auto
+
+  moreover from calculation have "mkAssign vs (a - {dash (assign_var v)}) \<in> WF_RELATION"
+    by simp
+
+  moreover from calculation have "assign_value v \<in> WF_ALPHA_EXPR" "assign_var v \<in> UNDASHED"
+    by auto
+
+  moreover from calculation have "\<alpha>e (VarE (dash (assign_var v))) \<subseteq> UNDASHED \<union> DASHED"
+    apply(safe)
+    apply(simp add:VarE_def)
+    apply(subgoal_tac "assign_var v \<in> UNDASHED")
+    apply(simp add:dash_def UNDASHED_def DASHED_def)
+    apply(simp)
+  done
+
+  moreover from calculation have "\<alpha>e (assign_value v) \<subseteq> UNDASHED \<union> DASHED"
+    by force
+        
+  moreover from calculation have "VarE (dash (assign_var v)) =p assign_value v \<in> WF_RELATION"
+    by (simp add:WF_RELATION_def)
+
+  ultimately show ?case
+    by (simp add:WF_RELATION_def)
+qed
+
+lemma AssignR_closure[simp]:
+"\<lbrakk> vs \<in> WF_ASSIGNMENT a; a \<in> WF_ALPHABET; a \<subseteq> UNDASHED \<union> DASHED; HOMOGENEOUS a \<rbrakk>
+   \<Longrightarrow> AssignR vs a \<in> WF_RELATION"
+  by (simp add:AssignR_def)
+
+theorem mkAssign_alphabet [simp] :
+"\<lbrakk> vs \<in> WF_ASSIGNMENT a; a \<in> WF_ALPHABET; a \<subseteq> UNDASHED \<union> DASHED \<rbrakk> \<Longrightarrow>
+ \<alpha> (mkAssign vs a) = homalph a"
+proof (induct vs arbitrary: a)
+  fix a
+  case Nil
+    thus ?case
+      by (simp add:SkipR_def)
+next        
+
+  case (Cons v vs)
+
+  moreover from calculation have "assign_value v \<in> WF_ALPHA_EXPR"
+    by (auto)
+
+  moreover from calculation have "a - {assign_var v} \<in> WF_ALPHABET" "vs \<in> WF_ASSIGNMENT (a - {dash (assign_var v)})" "a - {dash (assign_var v)} \<subseteq> UNDASHED \<union> DASHED"
+    by auto
+
+  moreover from calculation have "mkAssign vs (a - {dash (assign_var v)}) \<in> WF_RELATION"
+    by simp
+
+  moreover from calculation have "\<alpha> (mkAssign (v # vs) a) = \<alpha> (VarE (dash (assign_var v)) =p assign_value v) \<union> \<alpha> (mkAssign vs (a - {dash (assign_var v)}))"
+
+    apply(simp)
+
+      apply(subgoal_tac "(VarE (dash (assign_var v)) =p assign_value v) \<in> WF_ALPHA_PREDICATE")
+      apply(subgoal_tac "mkAssign vs (a - {dash (assign_var v)}) \<in> WF_ALPHA_PREDICATE")
+      apply(simp add:AndP_def)
+      apply(insert calculation)
+      apply(simp only:WF_RELATION_def)
+      apply(simp)
+      apply(simp)
+  done
+
+  moreover from calculation have "\<alpha> (VarE (dash (assign_var v)) =p assign_value v) = {dash (assign_var v)}\<union>\<alpha>e (assign_value v)"
+    by simp
+
+  moreover from calculation have "\<alpha> (VarE (dash (assign_var v)) =p assign_value v) \<subseteq> a"
+    by auto
+
+  moreover from calculation have "\<alpha> (mkAssign vs (a - {dash (assign_var v)})) = homalph (a - {dash (assign_var v)})"
+    by auto
+
+
+  moreover from calculation have "a \<subseteq> homalph a"
+    by (metis homalpha_subset)
+
+  moreover from calculation have "dash (assign_var v) \<in> homalph a"
+    by (smt Un_insert_left insert_subset subset_trans)
+
+  moreover from calculation have "\<alpha>e (assign_value v) \<subseteq> homalph a"
+    apply(subgoal_tac "\<alpha>e (assign_value v) \<subseteq> a")
+    apply(metis subset_trans)
+    apply(auto)
+  done
+
+  moreover from calculation have "\<alpha> (mkAssign (v # vs) a) \<subseteq> homalph a"
+    apply(simp)
+    apply(rule homalpha_mono)
+    apply(force)
+  done
+    
+  moreover from calculation have "homalph a \<subseteq> \<alpha> (mkAssign (v # vs) a)"
+    proof -
+      have r0:"dash (assign_var v) \<in> out (homalph a)"
+        by (metis Un_iff in_alphabet_ndash calculation(15) homalph_def homalph_in homalph_out)
+
+      with calculation have r1:"homalph a = in (homalph a) \<union> (out (homalph a) - {dash (assign_var v)}) \<union> {dash (assign_var v)}"
+      proof -
+        have "homalph a = in (homalph a) \<union> out (homalph a)"
+          by (metis homalpha_dashes in_out_complete)
+        also from r0 have "... = in (homalph a) \<union> (out (homalph a) - {dash (assign_var v)}) \<union> {dash (assign_var v)}"
+          by (force)
+        ultimately show ?thesis 
+          by metis
+      qed
+
+      have r2:"in (homalph a) \<subseteq> homalph (a - {dash (assign_var v)})"
+        apply(simp add:homalph_def)
+        apply(auto)
+        apply (metis DiffI IntE IntI image_empty image_insert in_alphabet_def in_dash)
+        sorry
+
+      have r3: "out (homalph a) - {dash (assign_var v)} \<subseteq> homalph (a - {dash (assign_var v)})"
+        apply(simp add:homalph_def)
+        apply(auto)
+        apply (metis VAR.out_undash_out equals0D)
+        apply (metis DiffI IntE IntI emptyE insertE out_alphabet_def)
+        sorry
+
+      have r4: "{dash (assign_var v)} \<subseteq> {dash (assign_var v)}"
+        by simp
+      
+      have r5: "(in (homalph a) \<union> (out (homalph a) - {dash (assign_var v)}) \<union> {dash (assign_var v)}) \<subseteq> ({dash (assign_var v)} \<union> \<alpha>e (assign_value v) \<union> homalph (a - {dash (assign_var v)}))"
+        by (smt Un_least Un_upper1 Un_upper2 r2 r3 subset_trans)
+
+
+      thus ?thesis
+        by (simp only:calculation, metis r1)
+        
+    qed
+
+  ultimately show ?case
+    by force
+qed      
+
+theorem AssignR_alphabet [simp] :
+"\<lbrakk> vs \<in> WF_ASSIGNMENT a; a \<in> WF_ALPHABET; a \<subseteq> UNDASHED \<union> DASHED; HOMOGENEOUS a \<rbrakk> \<Longrightarrow>
+ \<alpha> (AssignR vs a) = a"
+  by (simp add:AssignR_def homogeneous_homalpha)
+
+
+
 theorem WF_RELATION_TrueP [simp] :
 "\<lbrakk>a \<in> WF_ALPHABET;
  a \<subseteq> UNDASHED \<union> DASHED\<rbrakk> \<Longrightarrow>
@@ -256,41 +689,379 @@ done
 
 subsection {* Proof Experiments *}
 
-theorem
-"\<lbrakk>r \<in> WF_RELATION;
- a \<in> WF_ALPHABET;
- a \<subseteq> UNDASHED \<union> DASHED;
- COMPOSABLE a (\<alpha> r)\<rbrakk> \<Longrightarrow>
- false a ; r = false ((in a) \<union> out (\<alpha> r))"
-apply (utp_pred_eq_tac)
-apply (auto)
--- {* TODO: See if the proof of the subgoals can be automated. *}
-oops
+(* Convert this into a decent set of lemmas in the right place *)
+lemma dashed_twice_override:
+"\<lbrakk> p \<in> WF_RELATION; bq \<in> WF_BINDING; bp \<in> \<beta> p; a \<subseteq> DASHED_TWICE \<rbrakk> \<Longrightarrow>
+ bp \<oplus> bq on a \<in> \<beta> p"
+  apply(auto simp add:WF_RELATION_def)
+  apply(subgoal_tac "bp \<cong> (bp \<oplus> bq on a) on \<alpha> p")
+  apply(subgoal_tac "bp \<oplus> bq on a \<in> WF_BINDING")
+  apply(auto intro:beta_equiv_bindings)
+apply (metis WF_BINDING_override WF_BINDING_predicate)
+apply(subgoal_tac "\<alpha> p \<inter> a = {}")
+apply (metis Int_commute beta_equiv_comm beta_equiv_override_2)
+apply(simp add:DASHED_def UNDASHED_def DASHED_TWICE_def Un_def)
+apply (smt Collect_def disjoint_iff_not_equal in_mono mem_def)
+done
 
-theorem SemiR_assoc:
-assumes assm:
-  "r1 \<in> WF_RELATION"
-  "r2 \<in> WF_RELATION"
-  "r3 \<in> WF_RELATION"
-  "COMPOSABLE (\<alpha> r1) (\<alpha> r2)"
-  "COMPOSABLE (\<alpha> r2) (\<alpha> r3)"
-shows "r1 ; (r2 ; r3) = (r1 ; r2) ; r3"
-proof -
-  from assm have r1 :
-    "r1 ; r2 \<in> WF_RELATION"
-    "r2 ; r3 \<in> WF_RELATION"
-      by (simp_all)
+(* Show that the two versions of sequential composition are equal *)
+theorem SemiR_SemiB:
+  assumes "p \<in> WF_RELATION" "q \<in> WF_RELATION" "COMPOSABLE (\<alpha> p) (\<alpha> q)"
+  shows "p ; q = p ;\<^sub>B q"
+proof
+  (* First we show that the two alphabets are equal *)
+  from assms have salpha: "\<alpha> (p ; q) = in (\<alpha> p) \<union> out (\<alpha> q)"
+    by simp
 
-  from assm have r2 :
-    "COMPOSABLE (\<alpha> r1) (\<alpha> (r2 ; r3))"
-    "COMPOSABLE (\<alpha> (r1 ; r2)) (\<alpha> r3)"
-      by (auto elim! : COMPOSABLE_elim)
+  from assms show "\<alpha> (p ; q) = \<alpha> (p ;\<^sub>B q)"
+    by (simp add:SemiB_def)
 
-  from r1 r2 assm show ?thesis
-    apply(utp_pred_eq_tac)
-    apply(safe)
--- {* This seems difficult to prove, use algebraic approach instead. *}
-    sorry
+  from assms have comp: "dash ` dash ` in (\<alpha> q) = dash ` out (\<alpha> p)"
+    by (simp add:COMPOSABLE_def)
+
+  from assms have preds: "p \<in> WF_ALPHA_PREDICATE" "q \<in> WF_ALPHA_PREDICATE"
+    by (simp_all add:WF_RELATION_def)
+
+  (* We prove equivalence of the bindings by two inequalities *)
+  from assms show "bindings (p ; q) = bindings (p ;\<^sub>B q)"
+  proof (rule_tac subset_antisym)
+    (* \<beta> (p ; q) \<subseteq> \<beta> (p ;\<^sub>B q) *)
+
+   from assms preds salpha show "\<beta> (p ; q) \<subseteq> \<beta> (p ;\<^sub>B q)"
+   proof (simp add:SemiB_def SemiR_def ExistsResP_def ResP_def, simp add: AndP_def, simp add: SubstP_def, auto)
+     from assms have "dash ` out (\<alpha> p) \<in> WF_ALPHABET"
+       by auto
+
+     fix bp bq bx
+
+     assume assms':
+       "bp \<in> \<beta> p" "bq \<in> \<beta> q" "bx \<in> WF_BINDING" 
+       "SubstB SS2 bq \<cong> bx on in (\<alpha> p) \<union> out (\<alpha> q)"
+       "SubstB SS1 bp = SubstB SS2 bq"
+
+     from preds assms' have binds: "bp \<in> WF_BINDING" "bq \<in> WF_BINDING"
+       by (auto simp add:WF_ALPHA_PREDICATE_def WF_BINDING_SET_def)
+
+     have adashes: "in (\<alpha> p) \<subseteq> UNDASHED" "out (\<alpha> q) \<subseteq> DASHED"
+       by (auto simp add:in_alphabet_def out_alphabet_def)
+
+     from assms' binds adashes have bxbp: "bx \<cong> bp on in (\<alpha> p)"
+       by (metis SubstB_SS1_beta_equiv beta_equiv_comm beta_equiv_union)
+
+     from assms' binds adashes have bxbq: "bx \<cong> bq on out (\<alpha> q)"
+       by (metis SubstB_SS2_beta_equiv beta_equiv_comm beta_equiv_union)
+
+     from bxbp bxbq have bxover: "bx = (bx \<oplus> bp on in (\<alpha> p)) \<oplus> bq on out (\<alpha> q)"
+       by (metis beta_equiv_override)
+
+     moreover from assms' binds have "\<forall>x\<in>in (\<alpha> q). bp (dash x) = bq x"
+     proof (auto simp add:SubstB_def)
+       fix x
+       assume assms'': "x \<in> in (\<alpha> q)" "bp \<circ> inv SS1 = bq \<circ> inv SS2"
+       hence dash2: "dash (dash (x)) \<in> DASHED_TWICE"
+         by (simp add:dash_def in_alphabet_def UNDASHED_def DASHED_TWICE_def)
+
+       from assms'' have "bp (inv SS1 (dash (dash x))) = bq (inv SS2 (dash (dash x)))"
+         by (simp add:fun_eq_iff)
+
+       with assms'' show "bp (dash x) = bq x"
+         by (metis SS1_inv_d2 SS2_inv_d2 dash2 undash_dash)
+     qed
+
+     ultimately show "\<exists> b1 b2 b.
+                bx = (b \<oplus> b1 on in (\<alpha> p)) \<oplus> b2 on out (\<alpha> q) \<and>
+                b1 \<in> \<beta> p \<and>
+                b2 \<in> \<beta> q \<and> b \<in> WF_BINDING \<and> (\<forall>x\<in>in (\<alpha> q). b1 (dash x) = b2 x)"
+       by (metis assms')
+   qed
+
+   (* \<beta> (p ;\<^sub>B q) \<subseteq> \<beta> (p ; q) *)
+
+   from assms preds salpha show "\<beta> (p ;\<^sub>B q) \<subseteq> \<beta> (p ; q)"
+   proof (simp add:SemiB_def SemiR_def ExistsResP_def ResP_def, simp add: AndP_def, simp add: SubstP_def, auto)
+     fix bp bq bx
+     assume assms': "bp \<in> \<beta> p" "bq \<in> \<beta> q" "bx \<in> WF_BINDING" "\<forall>x\<in>in (\<alpha> q). bp (dash x) = bq x"
+
+     from preds assms' have binds: "bp \<in> WF_BINDING" "bq \<in> WF_BINDING"
+       by (auto simp add:WF_ALPHA_PREDICATE_def WF_BINDING_SET_def)
+     
+     with preds show "(bx \<oplus> bp on in (\<alpha> p)) \<oplus> bq on out (\<alpha> q) \<in> WF_BINDING"
+       by (metis WF_BINDING_override assms')
+
+    from assms' have "SubstB SS1 bp \<in> SubstB SS1 ` \<beta> p"
+      by auto
+
+    have inbp: "(bx \<oplus> SubstB SS1 bp on SS1 ` \<alpha> p) \<oplus> SubstB SS2 bq on SS2 ` \<alpha> q
+          \<in> SubstB SS1 ` \<beta> p"
+    proof -
+
+      have "(SubstB SS1 bx \<oplus> bp on \<alpha> p) \<oplus> SubstB SS1 bq on SS1 ` out (\<alpha> q) \<in> \<beta> p"
+        by (smt SS1_VAR_SUBST SS1_dashed SubstB_closure assms' assms bindings_override binds dashed_twice_override out_undashed override_on_comm preds)
+      
+      also have " ((bx \<oplus> SubstB SS1 bp on SS1 ` \<alpha> p) \<oplus> SubstB SS2 bq on SS2 ` \<alpha> q)
+                = (SubstB SS1 ((SubstB SS1 bx \<oplus> bp on \<alpha> p) \<oplus> SubstB SS1 bq on SS1 ` out (\<alpha> q)))"
+
+        by (smt SS1_SS2_alpha_union1 SS1_SS2_overlap SS1_VAR_SUBST SS2_dashes SS2_override_out' SubstB_closure SubstB_invol SubstB_override1 WF_ALPHABET_out WF_BINDING_override WF_RELATION_UNDASHED_DASHED WF_RELATION_alphabet assms' assms beta_equiv_override binds SS1_SubstB override_on_assoc preds)
+
+    ultimately show ?thesis
+      by (metis imageI)
+  qed
+
+  have inbq:"(bx \<oplus> SubstB SS1 bp on SS1 ` \<alpha> p) \<oplus> SubstB SS2 bq on SS2 ` \<alpha> q \<in> SubstB SS2 ` \<beta> q"
+  proof -
+    have b1:"(SubstB SS2 bx \<oplus> SubstB SS2 bp on SS2 ` in (\<alpha> p)) \<in> WF_BINDING"
+      by (metis SS2_VAR_SUBST SubstB_closure WF_BINDING_override assms'(3) binds(1))
+
+    then have "(SubstB SS2 bx \<oplus> SubstB SS2 bp on SS2 ` in (\<alpha> p)) \<oplus> bq on (\<alpha> q) \<in> \<beta> q"
+      by (metis WF_BINDING_override assms'(2) beta_equiv_bindings beta_equiv_override_3 beta_equiv_refl binds(2) preds(2))
+
+
+    also have " ((bx \<oplus> SubstB SS1 bp on SS1 ` \<alpha> p) \<oplus> SubstB SS2 bq on SS2 ` \<alpha> q)
+              = SubstB SS2 ((SubstB SS2 bx \<oplus> SubstB SS2 bp on SS2 ` in (\<alpha> p)) \<oplus> bq on (\<alpha> q))"
+      by (smt SS1_SS2_alpha_union2 SS1_override_in' SS2_SubstB SS2_VAR_SUBST SubstB_closure SubstB_override1 WF_ALPHABET_in WF_BINDING_override WF_RELATION_UNDASHED_DASHED WF_RELATION_alphabet assms' assms binds override_on_assoc override_on_cancel6 preds)
+    
+
+ 
+(*
+sledgehammer min [z3] (SS1_SS2_alpha_union1 SS1_SS2_alpha_union2 SS1_SS2_overlap SS1_VAR_SUBST SS1_invol SS1_dashes SS1_override_in' SS2_VAR_SUBST SS2_invol SS2_dashes SS2_override_out' SS2_SubstB SubstB_closure SubstB_invol SubstB_override1 SubstB_override2 WF_ALPHABET_image WF_ALPHABET_in WF_ALPHABET_out WF_BINDING_override WF_RELATION_UNDASHED_DASHED WF_RELATION_alphabet assms' assms beta_equiv_override binds image_compose image_id override_on_assoc override_on_comm preds out_undashed bindings_override override_on_cancel5 override_on_cancel6)
+
+*)
+
+    ultimately show ?thesis
+      by (metis imageI)
+
+  qed
+      
+  from assms assms' have eqt:"(bx \<oplus> SubstB SS1 bp on SS1 ` \<alpha> p) \<oplus> SubstB SS2 bq on SS2 ` \<alpha> q \<cong> (bx \<oplus> bp on in (\<alpha> p)) \<oplus> bq on out (\<alpha> q) on in (\<alpha> p) \<union> out (\<alpha> q)"
+    apply(auto intro!:beta_equiv_override_intro1 beta_equiv_override_intro1 [THEN beta_equiv_comm] beta_equiv_refl)
+    apply(auto intro:beta_equiv_empty simp add:WF_RELATION_def)
+    apply(rule_tac SS1_beta_equiv_in)
+    apply(auto)
+    apply(rule_tac SS2_beta_equiv_out)
+    apply(auto)
+  done
+    
+
+
+  from assms' show "\<exists>b1a\<in>SubstB SS1 ` \<beta> p \<inter> SubstB SS2 ` \<beta> q.
+    b1a \<cong> (bx \<oplus> bp on in (\<alpha> p)) \<oplus> bq on out (\<alpha> q) on in (\<alpha> p) \<union> out (\<alpha> q)"
+    apply(rule_tac x="(bx \<oplus> (SubstB SS1 bp) on (SS1 ` \<alpha> p)) \<oplus> (SubstB SS2 bq) on (SS2 ` \<alpha> q)" in bexI)
+    apply(auto simp add:inbp inbq eqt)
+
+  done
+
+  qed
+  qed
 qed
+
+lemma SemiB_assoc:
+  assumes "p \<in> WF_RELATION" "q \<in> WF_RELATION" "r \<in> WF_RELATION" 
+          "COMPOSABLE (\<alpha> p) (\<alpha> q)" "COMPOSABLE (\<alpha> q) (\<alpha> r)" 
+  shows "p ;\<^sub>B (q ;\<^sub>B r) = (p ;\<^sub>B q) ;\<^sub>B r"
+proof -
+  from assms have alphas1: "\<alpha> p \<in> WF_ALPHABET" "\<alpha> q \<in> WF_ALPHABET" "\<alpha> r \<in> WF_ALPHABET"
+    apply(simp_all only:WF_RELATION_def WF_ALPHA_PREDICATE_def)
+    apply(auto)
+  done
+
+  from assms have alphas2: "\<alpha> (p ;\<^sub>B q) \<in> WF_ALPHABET" "\<alpha> (q ;\<^sub>B r) \<in> WF_ALPHABET"
+    by (simp_all add:SemiB_wfalpha)
+
+  from alphas1 alphas2 assms have comps:"COMPOSABLE (\<alpha> p) (\<alpha> (q ;\<^sub>B r))" 
+                                        "COMPOSABLE (\<alpha> (p ;\<^sub>B q)) (\<alpha> r)"
+    apply(simp_all add:COMPOSABLE_def SemiB_def)
+    apply(auto simp add:in_alphabet_def dash_def out_alphabet_def)
+  done
+   
+  from assms have closed: "p ;\<^sub>B q \<in> WF_RELATION" "q ;\<^sub>B r \<in> WF_RELATION"
+    by (auto intro:SemiB_closure)
+ 
+  show ?thesis
+  proof
+
+    show "\<beta> (p ;\<^sub>B (q ;\<^sub>B r)) = \<beta> ((p ;\<^sub>B q) ;\<^sub>B r)"
+    proof
+          
+      from assms alphas1 comps closed show "\<beta> (p ;\<^sub>B (q ;\<^sub>B r)) \<subseteq> \<beta> ((p ;\<^sub>B q) ;\<^sub>B r)"
+        apply(auto simp add:SemiB_def)
+        apply(rule_tac x="(b \<oplus> b1 on in (\<alpha> p)) \<oplus> b1a on out (\<alpha> q)" in exI)
+        apply(rule_tac x="b2a" in exI)
+        apply(rule_tac x="b" in exI)
+        apply(auto)
+        apply (metis override_on_cancel6 override_out_in)
+        apply(rule_tac x="b1" in exI)
+        apply(rule_tac x="b1a" in exI)
+        apply(rule_tac x="b" in exI)
+        apply(auto)
+        apply(subgoal_tac "x \<notin> out (\<alpha> r)")
+        apply(simp)
+        apply(subgoal_tac "in (\<alpha> p) \<inter> out (\<alpha> r) = {}")
+        apply (metis (no_types) disjoint_iff_not_equal in_out_disj)
+        apply (metis in_out_disj)
+      done
+          
+    next
+
+      from assms alphas1 comps closed show "\<beta> ((p ;\<^sub>B q) ;\<^sub>B r) \<subseteq> \<beta> (p ;\<^sub>B (q ;\<^sub>B r))"
+        apply(auto simp add:SemiB_def)
+        apply(rule_tac x="b1a" in exI)
+        apply(rule_tac x="(b \<oplus> b2a on in (\<alpha> q)) \<oplus> b2 on out (\<alpha> r)" in exI) 
+        apply(rule_tac x="b" in exI)
+        apply(auto)
+        apply (metis override_on_cancel6 override_out_in)
+        apply(rule_tac x="b2a" in exI)
+        apply(rule_tac x="b2" in exI)
+        apply(rule_tac x="b" in exI)
+        apply(auto)
+        apply(subgoal_tac "x \<notin> out (\<alpha> r)") 
+        apply(simp)
+        apply (metis IntI equals0D in_out_disj)
+      done
+    qed
+  next
+
+    from assms alphas1 comps closed show "\<alpha> (p ;\<^sub>B q ;\<^sub>B r) = \<alpha> ((p ;\<^sub>B q) ;\<^sub>B r)"
+      by (simp add:SemiB_def)
+
+  qed
+qed
+
+lemma SemiR_assoc:
+  assumes "p \<in> WF_RELATION" "q \<in> WF_RELATION" "r \<in> WF_RELATION" 
+          "COMPOSABLE (\<alpha> p) (\<alpha> q)" "COMPOSABLE (\<alpha> q) (\<alpha> r)" 
+  shows "p ; (q ; r) = (p ; q) ; r"
+proof -
+  from assms have c1:"COMPOSABLE (\<alpha> p) (\<alpha> (q ; r))"
+    by (simp add:COMPOSABLE_def)
+
+  from assms have c2:"COMPOSABLE (\<alpha> (p ; q)) (\<alpha> r)"
+    apply(simp add:COMPOSABLE_def)
+    apply(metis out_alphabet_out)
+  done
+
+  have "p ; (q ; r) = p ;\<^sub>B (q ;\<^sub>B r)"
+    by (metis SemiR_SemiB SemiR_closure assms c1)
+
+  also have "... = (p ;\<^sub>B q) ;\<^sub>B r"
+    by (metis SemiB_assoc assms)
+
+  also have "... = (p ; q) ; r"
+    by (metis SemiR_SemiB SemiR_closure assms c2)
+
+  ultimately show ?thesis
+    by simp
+qed
+ 
+theorem SemiR_left_anhil:
+ assumes assm: "r \<in> WF_RELATION" "a \<in> WF_ALPHABET" "a \<subseteq> UNDASHED \<union> DASHED" "COMPOSABLE a (\<alpha> r)"
+ shows "false a ; r = false ((in a) \<union> out (\<alpha> r))"
+  by (insert assm, utp_pred_eq_tac) (auto simp add:WF_RELATION_def)
+
+theorem SemiR_right_anhil:
+ assumes assm: "r \<in> WF_RELATION" "a \<in> WF_ALPHABET" "a \<subseteq> UNDASHED \<union> DASHED" "COMPOSABLE (\<alpha> r) a"
+ shows "r ; false a = false ((out a) \<union> in (\<alpha> r))"
+  by (insert assm, utp_pred_eq_tac) (auto simp add:WF_RELATION_def)
+
+theorem SemiR_left_ident:
+ assumes assm: "r \<in> WF_RELATION" "a \<in> WF_ALPHABET" "a \<subseteq> UNDASHED \<union> DASHED" "HOMOGENEOUS a" "COMPOSABLE a (\<alpha> r)"
+ shows "\<Pi> a ; r = r"
+proof -
+  note assm
+  moreover 
+  from assm have "(\<Pi> a ; r) \<in> WF_RELATION"
+    by (simp)
+
+  moreover
+  from assm have "\<alpha> (\<Pi> a ; r) = \<alpha> r"
+    apply(simp add:COMPOSABLE_def HOMOGENEOUS_def)
+    apply (metis in_out_complete undash_dash' WF_RELATION_UNDASHED_DASHED)
+  done
+
+  moreover have "\<beta> (\<Pi> a ; r) = \<beta> r"
+  proof
+    from assm show "\<beta> (\<Pi> a ; r) \<subseteq> \<beta> r"
+    apply(simp add:SemiR_SemiB SemiB_def)
+    apply(simp add:SkipR_def LiftP_def)
+    apply(auto)
+    proof -
+      fix b1 b2 b
+      assume assm': "b1 \<in> WF_BINDING" "\<forall>x\<in>in a \<union> undash ` out a. b1 x = b1 (dash x)" 
+             "b2 \<in> \<beta> r" "b \<in> WF_BINDING" "\<forall>x\<in>in (\<alpha> r). b1 (dash x) = b2 x"
+
+      moreover from assms have "in a = in (\<alpha> r)"
+        apply(simp add:HOMOGENEOUS_def COMPOSABLE_def)
+        apply(metis undash_dash')
+      done
+        
+      moreover from assms have "\<alpha> r \<subseteq> UNDASHED \<union> DASHED"
+        by (simp add:WF_RELATION_def)
+
+      moreover from calculation have "(b \<oplus> b1 on in (\<alpha> r)) \<oplus> b2 on out (\<alpha> r) \<cong> b2 on \<alpha> r"
+      proof -
+        note calculation
+        moreover from calculation have "b1 \<cong> b2 on in (\<alpha> r)"
+          by (metis UnI1 beta_equiv_def)
+
+        moreover from calculation have "(b \<oplus> b1 on in (\<alpha> r)) \<oplus> b2 on out (\<alpha> r) = b \<oplus> (b1 \<oplus> b2 on out (\<alpha> r)) on \<alpha> r"
+          by (metis in_out_complete override_on_assoc)
+
+        ultimately show "(b \<oplus> b1 on in (\<alpha> r)) \<oplus> b2 on out (\<alpha> r) \<cong> b2 on \<alpha> r"
+          by (smt beta_equiv_comm beta_equiv_override beta_equiv_override_3 beta_equiv_refl beta_equiv_union in_out_complete override_out_in)
+      qed
+
+      ultimately show "(b \<oplus> b1 on in a) \<oplus> b2 on out (\<alpha> r) \<in> \<beta> r"
+        by (smt WF_BINDING_bindings WF_BINDING_override WF_RELATION_WF_ALPHA_PREDICATE beta_equiv_bindings beta_equiv_comm in_mono assm(1))
+    qed
+  
+  next
+    from assm show "\<beta> r \<subseteq> \<beta> (\<Pi> a ; r)"
+    apply(simp add:SemiR_SemiB SemiB_def)
+    apply(simp add:SkipR_def LiftP_def)
+    apply(auto)
+    proof -
+      fix br
+      assume br:"br \<in> \<beta> r"
+
+      let ?b  = "br" and
+          ?b1 = "\<lambda> x. if (x \<in> in a) then br x else if (x \<in> out a) then br (undash x) else br x" and
+          ?b2 = "br"
+
+      note br
+
+      moreover from br have brwf:"br \<in> WF_BINDING"
+        by (metis WF_BINDING_predicate WF_RELATION_WF_ALPHA_PREDICATE assm(1))
+
+      moreover with assm have b1wf:"?b1 \<in> WF_BINDING"
+        apply(auto simp add:WF_BINDING_def COMPOSABLE_def HOMOGENEOUS_def)
+        apply(simp add:dash_def)
+      done 
+
+      moreover have "?b1 \<cong> ?b2 on in a"
+        by (simp add:beta_equiv_def)
+
+      moreover then have "br = (?b \<oplus> ?b1 on in a) \<oplus> ?b2 on out (\<alpha> r)"
+        by (smt beta_equiv_comm beta_equiv_override override_on_idem)
+
+      moreover from assm have "\<forall>x\<in>in a \<union> undash ` out a. ?b1 x = ?b1 (dash x)"
+        by (auto simp add:COMPOSABLE_def HOMOGENEOUS_def)
+
+      ultimately show "\<exists>b1 b2 b.
+              br = (b \<oplus> b1 on in a) \<oplus> b2 on out (\<alpha> r) \<and>
+              b1 \<in> WF_BINDING \<and>
+              (\<forall>x\<in>in a \<union> undash ` out a. b1 x = b1 (dash x)) \<and>
+              b2 \<in> \<beta> r \<and> b \<in> WF_BINDING \<and> (\<forall>x\<in>in (\<alpha> r). b1 (dash x) = b2 x)"
+        using assms 
+        apply(rule_tac x="?b1" in exI)
+        apply(rule_tac x="?b2" in exI)
+        apply(rule_tac x="?b" in exI)
+        apply(force)
+      done
+    qed
+  qed
+
+  ultimately show ?thesis
+    by (metis pairI)
+qed
+      
 end
 end
