theories/generic/utp_expression.thy
@@ -1,0 +1,106 @@
+(******************************************************************************)
+(* Project: Deep Mechanisation of the UTP                                     *)
+(* File: utp/generic/utp_expression.thy                                       *)
+(* Author: Simon Foster and Frank Zeyda, University of York                   *)
+(******************************************************************************)
+
+header {* Generic Expressions *}
+
+theory utp_expression
+imports "../utp_types" utp_gen_pred utp_eval_tactic utp_value
+begin
+
+type_synonym ('VALUE, 'TYPE) EXPRESSION =
+  "(('VALUE, 'TYPE) BINDING \<Rightarrow> 'VALUE option) \<times> 'TYPE"
+
+type_synonym ('VALUE, 'TYPE) ALPHA_EXPRESSION =
+  "('TYPE ALPHABET) \<times> ('VALUE, 'TYPE) EXPRESSION"
+
+abbreviation expr_body :: "('VALUE, 'TYPE) ALPHA_EXPRESSION \<Rightarrow> (('VALUE, 'TYPE) BINDING \<Rightarrow> 'VALUE option)" where
+"expr_body x \<equiv> fst (snd x)"
+
+abbreviation expr_type :: "('VALUE, 'TYPE) ALPHA_EXPRESSION \<Rightarrow> 'TYPE" where
+"expr_type x \<equiv> snd (snd x)"
+
+abbreviation expr_alpha :: "('VALUE, 'TYPE) ALPHA_EXPRESSION \<Rightarrow> ('TYPE ALPHABET)" where
+"expr_alpha \<equiv> fst"
+
+notation expr_alpha ("\<alpha>e")
+
+context GEN_PRED
+begin
+
+subsection {* Expressions *}
+
+text {* We require expressions to be defined for well formed bindings. *}
+
+definition WF_ALPHA_EXPR :: "('VALUE, 'TYPE) ALPHA_EXPRESSION set" where
+"WF_ALPHA_EXPR \<equiv> {e. \<alpha>e e \<in> WF_ALPHABET 
+                   \<and> (\<forall> b \<in> WF_BINDING. \<exists> v. expr_body e b = Some v \<and> v : expr_type e)
+                   \<and> (\<forall> b1 \<in> WF_BINDING. \<forall> b2 \<in> WF_BINDING. 
+                      b1 \<cong> b2 on \<alpha>e e \<longrightarrow> expr_body e b1 = expr_body e b2)}"
+
+subsection {* Operators *}
+
+definition VarE :: "'TYPE VAR \<Rightarrow> ('VALUE, 'TYPE) ALPHA_EXPRESSION" where
+"VarE v \<equiv> ({v}, (\<lambda> b. Some (b v), var_type v))"
+
+subsection {* Predicates *}
+
+definition EqualP :: "('VALUE, 'TYPE) ALPHA_EXPRESSION \<Rightarrow> ('VALUE, 'TYPE) ALPHA_EXPRESSION \<Rightarrow> ('VALUE, 'TYPE) ALPHA_PREDICATE" where
+"e \<in> WF_ALPHA_EXPR \<and> f \<in> WF_ALPHA_EXPR \<longrightarrow> 
+ EqualP e f = (\<alpha>e e \<union> \<alpha>e f, {b. b \<in> WF_BINDING \<and> (expr_body e b = expr_body f b)})"
+
+notation EqualP (infixr "=p" 150)
+
+subsubsection {* Alphabet Theorems *}
+
+lemma VarP_alphabet [simp]: "\<alpha>e (VarE v) = {v}"
+  by (simp add:VarE_def)
+
+lemma EqualP_alphabet [simp]: 
+"\<lbrakk> e \<in> WF_ALPHA_EXPR; f \<in> WF_ALPHA_EXPR \<rbrakk> \<Longrightarrow> \<alpha> (e =p f) = \<alpha>e e \<union> \<alpha>e f"
+  by (simp add:EqualP_def)
+
+subsubsection {* Closure Theorems *}
+
+lemma VarE_closure[simp]:
+"VarE v \<in> WF_ALPHA_EXPR"
+  by (simp add:VarE_def WF_ALPHA_EXPR_def WF_BINDING_def beta_equiv_def)
+
+lemma EqualP_closure[simp]: 
+"\<lbrakk> e \<in> WF_ALPHA_EXPR; f \<in> WF_ALPHA_EXPR \<rbrakk> \<Longrightarrow>
+ e =p f \<in> WF_ALPHA_PREDICATE"
+  by (auto simp add:EqualP_def WF_ALPHA_EXPR_def WF_ALPHA_PREDICATE_def WF_BINDING_SET_def beta_equiv_union)
+  
+subsubsection {* Equality Theorems *}
+
+lemma EqualP_refl: "e \<in> WF_ALPHA_EXPR \<Longrightarrow> taut (e =p e)"
+  apply(insert EqualP_closure [where e="e" and f="e"])
+  apply(simp add:Tautology_def EqualP_def WF_ALPHA_PREDICATE_def TrueP_def)
+done
+
+lemma EqualP_sym: 
+"\<lbrakk> e \<in> WF_ALPHA_EXPR; f \<in> WF_ALPHA_EXPR; taut (e =p f)\<rbrakk> 
+ \<Longrightarrow> taut (f =p e)"
+  apply(insert EqualP_closure [where e="e" and f="f"])
+  apply(insert EqualP_closure [where e="f" and f="e"])
+  apply(simp add:Tautology_def EqualP_def WF_ALPHA_PREDICATE_def TrueP_def)
+  apply(force)
+done
+
+lemma EqualP_trans: 
+"\<lbrakk> e \<in> WF_ALPHA_EXPR; f \<in> WF_ALPHA_EXPR; g \<in> WF_ALPHA_EXPR; taut (e =p f); taut (f =p g)\<rbrakk> 
+ \<Longrightarrow> taut (e =p g)"
+  apply(insert EqualP_closure [where e="e" and f="f"])
+  apply(insert EqualP_closure [where e="f" and f="g"])
+  apply(insert EqualP_closure [where e="e" and f="g"])
+  apply(simp add:Tautology_def EqualP_def WF_ALPHA_PREDICATE_def TrueP_def)
+  apply(force)
+done
+
+declare EqualP_def [eval]
+declare VarE_def [eval]
+
+end
+end
